AbsInterp/Framework/Domains.lean
@@ -1,2 +1,3 @@
-import AbsInterp.Framework.Domains.Gamma
+import AbsInterp.Framework.Domains.Concretization
 import AbsInterp.Framework.Domains.Backward
+import AbsInterp.Framework.Domains.Interop.GaloisConnection
